src/Specific/Ed25519.v
@@ -1,5 +1,5 @@
 Require Import Bedrock.Word.
-Require Import Crypto.Spec.Ed25519.
+Require Import Crypto.Spec.EdDSA.
 Require Import Crypto.Tactics.VerdiTactics.
 Require Import BinNat BinInt NArith Crypto.Spec.ModularArithmetic.
 Require Import ModularArithmetic.ModularArithmeticTheorems.
@@ -10,13 +10,10 @@ Require Import Crypto.Spec.Encoding Crypto.Spec.ModularWordEncoding Crypto.Spec.
 Require Import Crypto.CompleteEdwardsCurve.ExtendedCoordinates.
 Require Import Crypto.CompleteEdwardsCurve.CompleteEdwardsCurveTheorems.
 Require Import Crypto.Util.IterAssocOp Crypto.Util.WordUtil Crypto.Rep.
-
-Local Infix "++" := Word.combine.
-Local Notation " a '[:' i ']' " := (Word.split1 i _ a) (at level 40).
-Local Notation " a '[' i ':]' " := (Word.split2 i _ a) (at level 40).
-Local Arguments H {_} _.
-Local Arguments scalarMultM1 {_} {_} _ _ _.
-Local Arguments unifiedAddM1 {_} {_} _ _.
+Require Import Coq.Setoids.Setoid.
+Require Import Coq.Classes.Morphisms.
+  
+(*TODO: move enerything before the section out of this file *)
 
 Local Ltac set_evars :=
   repeat match goal with
@@ -25,6 +22,21 @@ Local Ltac set_evars :=
 Local Ltac subst_evars :=
   repeat match goal with
          | [ e := ?E |- _ ] => is_evar E; subst e
+         end.
+
+Definition Let_In {A P} (x : A) (f : forall a : A, P a) : P x := let y := x in f y.
+Global Instance Let_In_Proper_nd {A P}
+  : Proper (eq ==> pointwise_relation _ eq ==> eq) (@Let_In A (fun _ => P)).
+Proof.
+  lazy; intros; congruence.
+Qed.
+
+Local Ltac replace_let_in_with_Let_In :=
+  repeat match goal with
+         | [ |- context G[let x := ?y in @?z x] ]
+           => let G' := context G[Let_In y z] in change G'
+         | [ |- _ = Let_In _ _ ]
+           => apply Let_In_Proper_nd; [ reflexivity | cbv beta delta [pointwise_relation]; intro ]
          end.
 
 Lemma funexp_proj {T T'} (proj : T -> T') (f : T -> T) (f' : T' -> T') x n
@@ -59,10 +71,6 @@ Proof.
            end. }
 Qed.
 
-Lemma B_proj : proj1_sig B = (fst(proj1_sig B), snd(proj1_sig B)). destruct B as [[]]; reflexivity. Qed.
-
-Require Import Coq.Setoids.Setoid.
-Require Import Coq.Classes.Morphisms.
 Global Instance option_rect_Proper_nd {A T}
   : Proper ((pointwise_relation _ eq) ==> eq  ==> eq ==> eq) (@option_rect A (fun _ => T)).
 Proof.
@@ -83,74 +91,6 @@ Proof.
   destruct v; reflexivity.
 Qed.
 
-Axiom decode_scalar : word b -> option N.
-Local Existing Instance Ed25519.FlEncoding.
-Axiom decode_scalar_correct : forall x, decode_scalar x = option_map (fun x : F (Z.of_nat Ed25519.l) => Z.to_N x) (dec x).
-
-Local Infix "==?" := E.point_eqb (at level 70) : E_scope.
-Local Infix "==?" := ModularArithmeticTheorems.F_eq_dec (at level 70) : F_scope.
-
-Lemma solve_for_R_eq : forall A B C, (A = B + C <-> B = A - C)%E.
-Proof.
-  intros; split; intros; subst; unfold E.sub;
-    rewrite <-E.add_assoc, ?E.add_opp_r, ?E.add_opp_l, E.add_0_r; reflexivity.
-Qed.
-
-Lemma solve_for_R : forall A B C, (A ==? B + C)%E = (B ==? A - C)%E.
-Proof.
-  intros.
-  repeat match goal with |- context [(?P ==? ?Q)%E] =>
-                      let H := fresh "H" in
-                      destruct (E.point_eq_dec P Q) as [H|H];
-                        (rewrite (E.point_eqb_complete _ _ H) || rewrite (E.point_eqb_neq_complete _ _ H))
-  end; rewrite solve_for_R_eq in H; congruence.
-Qed.
-
-Local Notation "'(' X ',' Y ',' Z ',' T ')'" := (mkExtended X Y Z T).
-Local Notation "2" := (ZToField 2) : F_scope.
-
-Local Existing Instance PointEncoding.
-Lemma decode_point_eq : forall (P_ Q_ : word (S (b-1))) (P Q:E.point),
-  dec P_ = Some P ->
-  dec Q_ = Some Q ->
-  weqb P_ Q_ = (P ==? Q)%E.
-Proof.
-  intros.
-  replace P_ with (enc P) in * by (auto using encoding_canonical).
-  replace Q_ with (enc Q) in * by (auto using encoding_canonical).
-  rewrite E.point_eqb_correct.
-  edestruct E.point_eq_dec; (apply weqb_true_iff || apply weqb_false_iff); congruence.
-Qed.
-
-Lemma decode_test_encode_test : forall S_ X, option_rect (fun _ : option E.point => bool)
- (fun S : E.point => (S ==? X)%E) false (dec S_) = weqb S_ (enc X).
-Proof.
-  intros.
-  destruct (dec S_) eqn:H.
-  { symmetry; eauto using decode_point_eq, encoding_valid. }
-  { simpl @option_rect.
-    destruct (weqb S_ (enc X)) eqn:Heqb; trivial.
-    apply weqb_true_iff in Heqb. subst. rewrite encoding_valid in H; discriminate. }
-Qed.
-
-Definition enc' : F q * F q -> word b.
-Proof.
-  intro x.
-  let enc' := (eval hnf in (@enc (@E.point curve25519params) _ _)) in
-  match (eval cbv [proj1_sig] in (fun pf => enc' (exist _ x pf))) with
-  | (fun _ => ?enc') => exact enc'
-  end.
-Defined.
-
-Definition enc'_correct : @enc (@E.point curve25519params) _ _ = (fun x => enc' (proj1_sig x))
-  := eq_refl.
-
-Definition Let_In {A P} (x : A) (f : forall a : A, P a) : P x := let y := x in f y.
-Global Instance Let_In_Proper_nd {A P}
-  : Proper (eq ==> pointwise_relation _ eq ==> eq) (@Let_In A (fun _ => P)).
-Proof.
-  lazy; intros; congruence.
-Qed.
 Lemma option_rect_function {A B C S' N' v} f
   : f (option_rect (fun _ : option A => option B) S' N' v)
     = option_rect (fun _ : option A => C) (fun x => f (S' x)) (f N') v.
@@ -169,13 +109,17 @@ Local Ltac commute_option_rect_Let_In := (* pull let binders out side of option_
       abstract (cbv [Let_In]; reflexivity)
     | ]
   end.
-Local Ltac replace_let_in_with_Let_In :=
-  repeat match goal with
-         | [ |- context G[let x := ?y in @?z x] ]
-           => let G' := context G[Let_In y z] in change G'
-         | [ |- _ = Let_In _ _ ]
-           => apply Let_In_Proper_nd; [ reflexivity | cbv beta delta [pointwise_relation]; intro ]
-         end.
+
+(** TODO: possibly move me, remove local *)
+Local Ltac replace_option_match_with_option_rect :=
+  idtac;
+  lazymatch goal with
+  | [ |- _ = ?RHS :> ?T ]
+    => lazymatch RHS with
+       | match ?a with None => ?N | Some x => @?S x end
+         => replace RHS with (option_rect (fun _ => T) S N a) by (destruct a; reflexivity)
+       end
+  end.
 Local Ltac simpl_option_rect := (* deal with [option_rect _ _ _ None] and [option_rect _ _ _ (Some _)] *)
   repeat match goal with
          | [ |- context[option_rect ?P ?S ?N None] ]
@@ -184,72 +128,255 @@ Local Ltac simpl_option_rect := (* deal with [option_rect _ _ _ None] and [optio
            => change (option_rect P S N (Some x)) with (S x); cbv beta
          end.
 
-Section Ed25519Frep.
-  Generalizable All Variables.
+Definition COMPILETIME {T} (x:T) : T := x.
+
+
+
+Lemma N_to_nat_le_mono : forall a b, (a <= b)%N -> (N.to_nat a <= N.to_nat b)%nat.
+Proof.
+  intros.
+  pose proof (Nomega.Nlt_out a (N.succ b)).
+  rewrite N2Nat.inj_succ, N.lt_succ_r, <-NPeano.Nat.lt_succ_r in *; auto.
+Qed.
+Lemma N_size_nat_le_mono : forall a b, (a <= b)%N -> (N.size_nat a <= N.size_nat b)%nat.
+Proof.
+  intros.
+  destruct (N.eq_dec a 0), (N.eq_dec b 0); try abstract (subst;rewrite ?N.le_0_r in *;subst;simpl;omega).
+  rewrite !Nsize_nat_equiv, !N.size_log2 by assumption.
+  edestruct N.succ_le_mono; eauto using N_to_nat_le_mono, N.log2_le_mono.
+Qed.
+
+Lemma Z_to_N_Z_of_nat : forall n, Z.to_N (Z.of_nat n) = N.of_nat n.
+Proof. induction n; auto. Qed.
+
+Lemma Z_of_nat_nonzero : forall m, m <> 0 -> (0 < Z.of_nat m)%Z.
+Proof. intros. destruct m; [congruence|reflexivity]. Qed.
+
+Lemma N_of_nat_modulo : forall n m, m <> 0 -> N.of_nat (n mod m)%nat = (N.of_nat n mod N.of_nat m)%N.
+Proof.
+  intros.
+  apply Znat.N2Z.inj_iff.
+  rewrite !Znat.nat_N_Z.
+  rewrite Zdiv.mod_Zmod by auto.
+  apply Znat.Z2N.inj_iff.
+  { apply Z.mod_pos_bound. apply Z_of_nat_nonzero. assumption. }
+  { apply Znat.N2Z.is_nonneg. }
+  rewrite Znat.Z2N.inj_mod by (auto using Znat.Nat2Z.is_nonneg, Z_of_nat_nonzero).
+  rewrite !Z_to_N_Z_of_nat, !Znat.N2Z.id; reflexivity.
+Qed.
+
+Lemma encoding_canonical' {T} {B} {encoding:canonical encoding of T as B} :
+  forall a b, enc a = enc b -> a = b.
+Proof.
+  intros.
+  pose proof (f_equal dec H).
+  pose proof encoding_valid.
+  pose proof encoding_canonical.
+  congruence.
+Qed.
+
+Lemma compare_encodings {T} {B} {encoding:canonical encoding of T as B}
+           (B_eqb:B->B->bool) (B_eqb_iff : forall a b:B, (B_eqb a b = true) <-> a = b)
+           : forall a b : T, (a = b) <-> (B_eqb (enc a) (enc b) = true).
+Proof.
+  intros.
+  split; intro H.
+  { rewrite B_eqb_iff; congruence. }
+  { apply B_eqb_iff in H; eauto using encoding_canonical'. }
+Qed.
+
+Lemma eqb_eq_dec' {T} (eqb:T->T->bool) (eqb_iff:forall a b, eqb a b = true <-> a = b) :
+    forall a b, if eqb a b then a = b else a <> b.
+Proof.
+  intros.
+  case_eq (eqb a b); intros.
+  { eapply eqb_iff; trivial. }
+  { specialize (eqb_iff a b). rewrite H in eqb_iff. intuition. }
+Qed.
+
+Definition eqb_eq_dec {T} (eqb:T->T->bool) (eqb_iff:forall a b, eqb a b = true <-> a = b) :
+  forall a b : T, {a=b}+{a<>b}.
+Proof.
+  intros.
+  pose proof (eqb_eq_dec' eqb eqb_iff a b).
+  destruct (eqb a b); eauto.
+Qed.
+
+Definition eqb_eq_dec_and_output {T} (eqb:T->T->bool) (eqb_iff:forall a b, eqb a b = true <-> a = b) :
+  forall a b : T, {a = b /\ eqb a b = true}+{a<>b /\ eqb a b = false}.
+Proof.
+  intros.
+  pose proof (eqb_eq_dec' eqb eqb_iff a b).
+  destruct (eqb a b); eauto.
+Qed. 
+
+Lemma eqb_compare_encodings {T} {B} {encoding:canonical encoding of T as B}
+           (T_eqb:T->T->bool) (T_eqb_iff : forall a b:T, (T_eqb a b = true) <-> a = b)
+           (B_eqb:B->B->bool) (B_eqb_iff : forall a b:B, (B_eqb a b = true) <-> a = b)
+           : forall a b : T, T_eqb a b = B_eqb (enc a) (enc b).
+Proof.
+  intros;
+    destruct (eqb_eq_dec_and_output T_eqb T_eqb_iff a b);
+    destruct (eqb_eq_dec_and_output B_eqb B_eqb_iff (enc a) (enc b));
+    intuition;
+    try find_copy_apply_lem_hyp B_eqb_iff;
+    try find_copy_apply_lem_hyp T_eqb_iff;
+    try congruence.
+    apply (compare_encodings B_eqb B_eqb_iff) in H2; congruence.
+Qed.
+
+Lemma decode_failed_neq_encoding {T B} (encoding_T_B:canonical encoding of T as B) (X:B)
+  (dec_failed:dec X = None) (a:T) : X <> enc a.
+Proof. pose proof encoding_valid. congruence. Qed.
+Lemma compare_without_decoding {T B} (encoding_T_B:canonical encoding of T as B)
+      (T_eqb:T->T->bool) (T_eqb_iff:forall a b, T_eqb a b = true <-> a = b)
+      (B_eqb:B->B->bool) (B_eqb_iff:forall a b, B_eqb a b = true <-> a = b)
+      (P_:B) (Q:T) : 
+  option_rect (fun _ : option T => bool)
+                 (fun P : T => T_eqb P Q)
+                 false
+              (dec P_)
+    = B_eqb P_ (enc Q).
+Proof.
+  destruct (dec P_) eqn:Hdec; simpl option_rect.
+  { apply encoding_canonical in Hdec; subst; auto using eqb_compare_encodings. }
+  { pose proof encoding_canonical.
+    pose proof encoding_valid.
+    pose proof eqb_compare_encodings.
+    eapply decode_failed_neq_encoding in Hdec.
+    destruct (B_eqb P_ (enc Q)) eqn:Heq; [rewrite B_eqb_iff in Heq; eauto | trivial]. }
+Qed.
+
+Generalizable All Variables.
+Section FSRepOperations.
+  Context {q:Z} {prime_q:Znumtheory.prime q} {two_lt_q:(2 < q)%Z}.
   Context `(rcS:RepConversions N SRep) (rcSOK:RepConversionsOK rcS).
-  Context `(rcF:RepConversions (F (Ed25519.q)) FRep) (rcFOK:RepConversionsOK rcF).
+  Context `(rcF:RepConversions (F q) FRep) (rcFOK:RepConversionsOK rcF).
   Context (FRepAdd FRepSub FRepMul:FRep->FRep->FRep) (FRepAdd_correct:RepBinOpOK rcF add FRepMul).
   Context (FRepSub_correct:RepBinOpOK rcF sub FRepSub) (FRepMul_correct:RepBinOpOK rcF mul FRepMul).
-  Local Notation rep2F := (unRep : FRep -> F (Ed25519.q)).
-  Local Notation F2Rep := (toRep : F (Ed25519.q) -> FRep).
-  Local Notation rep2S := (unRep : SRep -> N).
-  Local Notation S2Rep := (toRep : N -> SRep).
-
-  Axiom FRepOpp : FRep -> FRep.
-  Axiom FRepOpp_correct : forall x, opp (rep2F x) = rep2F (FRepOpp x).
-
-  Axiom wltu : forall {b}, word b -> word b -> bool.
-  Axiom wltu_correct : forall {b} (x y:word b), wltu x y = (wordToN x <? wordToN y)%N.
-
-  Axiom compare_enc : forall x y, F_eqb x y = weqb (@enc _ _ FqEncoding x) (@enc _ _ FqEncoding y).
-
-  Axiom wire2FRep : word (b-1) -> option FRep.
-  Axiom wire2FRep_correct : forall x, Fm_dec x = option_map rep2F (wire2FRep x).
-
-  Axiom FRep2wire : FRep -> word (b-1).
-  Axiom FRep2wire_correct : forall x, FRep2wire x = @enc _ _ FqEncoding (rep2F x).
-
   Axiom SRep_testbit : SRep -> nat -> bool.
   Axiom SRep_testbit_correct : forall (x0 : SRep) (i : nat), SRep_testbit x0 i = N.testbit_nat (unRep x0) i.
 
-  Definition FSRepPow x n := iter_op FRepMul (toRep 1%F) SRep_testbit n x 255.
-  Lemma FSRepPow_correct : forall x n, (N.size_nat (unRep n) <= 255)%nat -> (unRep x ^ unRep n)%F = unRep (FSRepPow x n).
+  Definition FSRepPow width x n := iter_op FRepMul (toRep 1%F) SRep_testbit n x width.
+  Lemma FSRepPow_correct : forall width x n, (N.size_nat (unRep n) <= width)%nat -> (unRep x ^ unRep n)%F = unRep (FSRepPow width x n).
   Proof. (* this proof derives the required formula, which I copy-pasted above to be able to reference it without the length precondition *)
     unfold FSRepPow; intros.
     erewrite <-pow_nat_iter_op_correct by auto.
-    erewrite <-(fun x => iter_op_spec (scalar := SRep) (mul (m:=Ed25519.q)) F_mul_assoc _ F_mul_1_l _ unRep SRep_testbit_correct n x 255%nat) by auto.
+    erewrite <-(fun x => iter_op_spec (scalar := SRep) mul F_mul_assoc _ F_mul_1_l _ unRep SRep_testbit_correct n x width) by auto.
     rewrite <-(rcFOK 1%F) at 1.
     erewrite <-iter_op_proj by auto.
     reflexivity.
   Qed.
 
-  Definition FRepInv x : FRep := FSRepPow x (S2Rep (Z.to_N (Ed25519.q - 2))).
-  Lemma FRepInv_correct : forall x, inv (rep2F x)%F = rep2F (FRepInv x).
-    unfold FRepInv; intros.
+  Definition FRepInv x : FRep := FSRepPow (COMPILETIME (N.size_nat (Z.to_N (q - 2)))) x (COMPILETIME (toRep (Z.to_N (q - 2)))).
+  Lemma FRepInv_correct : forall x, inv (unRep x)%F = unRep (FRepInv x).
+    unfold FRepInv, COMPILETIME; intros.
     rewrite <-FSRepPow_correct; rewrite rcSOK; try reflexivity.
     pose proof @Fq_inv_fermat_correct as H; unfold inv_fermat in H; rewrite H by
-        auto using Ed25519.prime_q, Ed25519.two_lt_q.
+        auto using prime_q, two_lt_q.
     reflexivity.
   Qed.
+End FSRepOperations.
+
+Section ESRepOperations.
+  Context {tep:TwistedEdwardsParams} {a_is_minus1:a = opp 1}.
+  Context `{rcS:RepConversions N SRep} {rcSOK:RepConversionsOK rcS}.
+  Context {SRep_testbit : SRep -> nat -> bool}.
+  Context {SRep_testbit_correct : forall (x0 : SRep) (i : nat), SRep_testbit x0 i = N.testbit_nat (unRep x0) i}.
+  Definition scalarMultExtendedSRep (bound:nat) (a:SRep) (P:extendedPoint) :=
+    unExtendedPoint (iter_op (@unifiedAddM1 _ a_is_minus1) (mkExtendedPoint E.zero) SRep_testbit a P bound).
+  Definition scalarMultExtendedSRep_correct : forall (bound:nat) (a:SRep) (P:extendedPoint) (bound_satisfied:(N.size_nat (unRep a) <= bound)%nat),
+      scalarMultExtendedSRep bound a P = (N.to_nat (unRep a) * unExtendedPoint P)%E.
+  Proof. (* derivation result copy-pasted to above to remove preconditions from it *)
+    intros.
+    rewrite <-(scalarMultM1_rep a_is_minus1), <-(@iter_op_spec _ extendedPoint_eq _ _ (@unifiedAddM1 _ a_is_minus1) _ (@unifiedAddM1_assoc _ a_is_minus1) _ (@unifiedAddM1_0_l _ a_is_minus1) _ _ SRep_testbit_correct _ _ bound) by assumption.
+    reflexivity.
+  Defined.
+End ESRepOperations.
+
+Section EdDSADerivation.
+  Context `(eddsaprm:EdDSAParams).
+  Context `(rcS:RepConversions N SRep) (rcSOK:RepConversionsOK rcS).
+  Context `(rcF:RepConversions (F q) FRep) (rcFOK:RepConversionsOK rcF).
+  Context (FRepAdd FRepSub FRepMul:FRep->FRep->FRep) (FRepAdd_correct:RepBinOpOK rcF add FRepMul).
+  Context (FRepSub_correct:RepBinOpOK rcF sub FRepSub) (FRepMul_correct:RepBinOpOK rcF mul FRepMul).
+  Context (FSRepPow:FRep->SRep->FRep) (FSRepPow_correct: forall x n, (N.size_nat (unRep n) <= (N.size_nat (N.of_nat l)))%nat -> (unRep x ^ unRep n)%F = unRep (FSRepPow x n)).
+  Context (FRepInv:FRep->FRep) (FRepInv_correct:forall x, inv (unRep x)%F = unRep (FRepInv x)).
+  Context (a_is_minus1:CompleteEdwardsCurve.a = opp 1).
+
+  Local Infix "++" := Word.combine.
+  Local Infix "==?" := E.point_eqb (at level 70) : E_scope.
+  Local Infix "==?" := ModularArithmeticTheorems.F_eq_dec (at level 70) : F_scope.
+  Local Notation " a '[:' i ']' " := (Word.split1 i _ a) (at level 40).
+  Local Notation " a '[' i ':]' " := (Word.split2 i _ a) (at level 40).
+  Local Arguments H {_ _} _.
+  Local Arguments unifiedAddM1 {_} {_} _ _.
+
+  (*TODO:move*)
+  Lemma F_eqb_iff : forall x y : F q, F_eqb x y = true <-> x = y.
+  Proof.
+    split; eauto using F_eqb_eq, F_eqb_complete.
+  Qed.
+  Lemma E_eqb_iff : forall x y : E.point, E.point_eqb x y = true <-> x = y.
+  Proof.
+    split; eauto using E.point_eqb_sound, E.point_eqb_complete.
+  Qed.
+  
+  Lemma B_proj : proj1_sig B = (fst(proj1_sig B), snd(proj1_sig B)). destruct B as [[]]; reflexivity. Qed.
+
+  Lemma solve_for_R_eq : forall A B C, (A = B + C <-> B = A - C)%E.
+  Proof.
+    intros; split; intros; subst; unfold E.sub;
+      rewrite <-E.add_assoc, ?E.add_opp_r, ?E.add_opp_l, E.add_0_r; reflexivity.
+  Qed.
+  
+  Lemma solve_for_R : forall A B C, (A ==? B + C)%E = (B ==? A - C)%E.
+  Proof.
+    intros;
+      rewrite !E.point_eqb_correct;
+      repeat match goal with |- context[E.point_eq_dec ?x ?y] => destruct (E.point_eq_dec x y) end;
+      rewrite solve_for_R_eq in *;
+      congruence.
+  Qed.
+
+  Axiom decode_scalar : word b -> option N.
+  Axiom decode_scalar_correct : forall x, decode_scalar x = option_map (fun x : F (Z.of_nat l) => Z.to_N x) (dec x).
+  
+  Axiom enc':(F q * F q) -> word b.
+  Axiom enc'_correct : @enc E.point _ _ = (fun x => enc' (proj1_sig x)).
+
+  Axiom FRepOpp : FRep -> FRep.
+  Axiom FRepOpp_correct : forall x, opp (unRep x) = unRep (FRepOpp x).
+
+  Axiom wltu : forall {b}, word b -> word b -> bool.
+  Axiom wltu_correct : forall {b} (x y:word b), wltu x y = (wordToN x <? wordToN y)%N.
+
+  Axiom wire2FRep : word (b-1) -> option FRep.
+  Axiom wire2FRep_correct : forall x, Fm_dec x = option_map unRep (wire2FRep x).
+
+  Axiom FRep2wire : FRep -> word (b-1).
+  Axiom FRep2wire_correct : forall x, FRep2wire x = @enc _ _ FqEncoding (unRep x).
+  
+  Local Notation "'(' X ',' Y ',' Z ',' T ')'" := (mkExtended X Y Z T).
+  Local Notation "2" := (ZToField 2) : F_scope.
 
   Lemma unfoldDiv : forall {m} (x y:F m), (x/y = x * inv y)%F. Proof. unfold div. congruence. Qed.
 
   Definition rep2E (r:FRep * FRep * FRep * FRep) : extended :=
-    match r with (((x, y), z), t) => mkExtended (rep2F x) (rep2F y) (rep2F z) (rep2F t) end.
+    match r with (((x, y), z), t) => mkExtended (unRep x) (unRep y) (unRep z) (unRep t) end.
 
   Lemma if_map : forall {T U} (f:T->U) (b:bool) (x y:T), (if b then f x else f y) = f (if b then x else y).
   Proof.
     destruct b; trivial.
   Qed.
 
-  Local Ltac Let_In_unRep :=
+  (** TODO: Move me *)
+  Local Ltac Let_In_app fn :=
     match goal with
-    | [ |- appcontext G[Let_In (unRep ?x) ?f] ]
-      => change (Let_In (unRep x) f) with (Let_In x (fun y => f (unRep y))); cbv beta
+    | [ |- appcontext G[Let_In (fn ?x) ?f] ]
+      => change (Let_In (fn x) f) with (Let_In x (fun y => f (fn y))); cbv beta
     end.
 
-
-  (** TODO: Move me *)
   Lemma pull_Let_In {B C} (f : B -> C) A (v : A) (b : A -> B)
     : Let_In v (fun v' => f (b v')) = f (Let_In v b).
   Proof.
@@ -266,11 +393,12 @@ Section Ed25519Frep.
       @Let_In _ (fun _ => T) (x, y) (fun p => f ((g1 (fst p), g2 (snd p)))).
   Proof. reflexivity. Qed.
 
+
   Create HintDb FRepOperations discriminated.
-  Hint Rewrite FRepMul_correct FRepAdd_correct FRepSub_correct FRepInv_correct FSRepPow_correct FRepOpp_correct : FRepOperations.
+  Hint Rewrite FRepMul_correct FRepAdd_correct FRepSub_correct @FRepInv_correct @FSRepPow_correct FRepOpp_correct : FRepOperations.
 
   Create HintDb EdDSA_opts discriminated.
-  Hint Rewrite FRepMul_correct FRepAdd_correct FRepSub_correct FRepInv_correct FSRepPow_correct FRepOpp_correct : EdDSA_opts.
+  Hint Rewrite FRepMul_correct FRepAdd_correct FRepSub_correct @FRepInv_correct @FSRepPow_correct FRepOpp_correct : EdDSA_opts.
 
   Lemma unifiedAddM1Rep_sig : forall a b : FRep * FRep * FRep * FRep, { unifiedAddM1Rep | rep2E unifiedAddM1Rep = unifiedAddM1' (rep2E a) (rep2E b) }.
   Proof.
@@ -285,7 +413,7 @@ Section Ed25519Frep.
     { etransitivity; [|replace_let_in_with_Let_In; reflexivity].
       repeat (
         autorewrite with FRepOperations;
-        Let_In_unRep;
+        Let_In_app unRep;
         eapply Let_In_Proper_nd; [reflexivity|cbv beta delta [Proper respectful pointwise_relation]; intro]).
         lazymatch goal with |- ?LHS = (unRep ?x, unRep ?y, unRep ?z, unRep ?t) =>
                             change (LHS = (rep2E (((x, y), z), t)))
@@ -302,7 +430,7 @@ Section Ed25519Frep.
   Definition unifiedAddM1Rep (a b:FRep * FRep * FRep * FRep) : FRep * FRep * FRep * FRep := Eval hnf in proj1_sig (unifiedAddM1Rep_sig a b).
   Definition unifiedAddM1Rep_correct a b : rep2E (unifiedAddM1Rep a b) = unifiedAddM1' (rep2E a) (rep2E b)  := Eval hnf in proj2_sig (unifiedAddM1Rep_sig a b).
 
-  Definition rep2T (P:FRep * FRep) := (rep2F (fst P), rep2F (snd P)).
+  Definition rep2T (P:FRep * FRep) := (unRep (fst P), unRep (snd P)).
   Definition erep2trep (P:FRep * FRep * FRep * FRep) := Let_In P (fun P => Let_In (FRepInv (snd (fst P))) (fun iZ => (FRepMul (fst (fst (fst P))) iZ, FRepMul (snd (fst (fst P))) iZ))).
   Lemma erep2trep_correct : forall P, rep2T (erep2trep P) = extendedToTwisted (rep2E P).
   Proof.
@@ -310,16 +438,15 @@ Section Ed25519Frep.
     rewrite !unfoldDiv, <-!FRepMul_correct, <-FRepInv_correct. reflexivity.
   Qed.
 
-  (** TODO: possibly move me, remove local *)
-  Local Ltac replace_option_match_with_option_rect :=
-    idtac;
-    lazymatch goal with
-    | [ |- _ = ?RHS :> ?T ]
-      => lazymatch RHS with
-         | match ?a with None => ?N | Some x => @?S x end
-           => replace RHS with (option_rect (fun _ => T) S N a) by (destruct a; reflexivity)
-         end
-    end.
+  Lemma Fl_SRep_bound : forall (a:F (Z.of_nat EdDSA.l)), (N.size_nat (unRep (toRep (Z.to_N (FieldToZ a)))) <= N.size_nat (Z.to_N (Z.pred (Z.of_nat EdDSA.l))))%nat.
+  Proof.
+    intros.
+    rewrite rcSOK.
+    apply N_size_nat_le_mono.
+    pose proof l_odd.
+    edestruct (FieldToZ_range a); [omega|].
+    apply Znat.Z2N.inj_le; trivial; omega.
+  Qed.
 
   (** TODO: Move me, remove Local *)
   Definition proj1_sig_unmatched {A P} := @proj1_sig A P.
@@ -336,17 +463,14 @@ Section Ed25519Frep.
     (* [proj1_sig_nounfold] is a thin wrapper around [proj1_sig]; unfolding it restores [proj1_sig].  Unfolding [proj1_sig_nounfold] exposes the pattern match, which is reduced by ι. *)
     cbv [proj1_sig_nounfold proj1_sig_unfold].
 
-  (** TODO: possibly move me, remove Local *)
-  Local Ltac reflexivity_when_unification_is_stupid_about_evars
-    := repeat first [ reflexivity
-                    | apply f_equal ].
+  Lemma unfold_E_sub : forall a b, (a - b = a + E.opp b)%E. Proof. reflexivity. Qed.
 
 
   Local Existing Instance eq_Reflexive. (* To get some of the [setoid_rewrite]s below to work, we need to infer [Reflexive eq] before [Reflexive Equivalence.equiv] *)
 
   (* TODO: move me *)
   Lemma fold_rep2E x y z t
-    : (rep2F x, rep2F y, rep2F z, rep2F t) = rep2E (((x, y), z), t).
+    : (unRep x, unRep y, unRep z, unRep t) = rep2E (((x, y), z), t).
   Proof. reflexivity. Qed.
   Lemma commute_negateExtended'_rep2E x y z t
     : negateExtended' (rep2E (((x, y), z), t))
@@ -356,7 +480,7 @@ Section Ed25519Frep.
     : (x, y, z, t) = rep2E (((toRep x, toRep y), toRep z), toRep t).
   Proof. simpl; rewrite !rcFOK; reflexivity. Qed.
   Lemma fold_rep2E_rrfr x y z t
-    : (rep2F x, rep2F y, z, rep2F t) = rep2E (((x, y), toRep z), t).
+    : (unRep x, unRep y, z, unRep t) = rep2E (((x, y), toRep z), t).
   Proof. simpl; rewrite !rcFOK; reflexivity. Qed.
   Lemma fold_rep2E_0fff y z t
     : (0%F, y, z, t) = rep2E (((toRep 0%F, toRep y), toRep z), toRep t).
@@ -369,45 +493,51 @@ Section Ed25519Frep.
       = rep2E (((FRepOpp x, y), toRep z), FRepOpp t).
   Proof. rewrite <- commute_negateExtended'_rep2E; simpl; rewrite !rcFOK; reflexivity. Qed.
 
-  Hint Rewrite @F_mul_0_l commute_negateExtended'_rep2E_rrfr fold_rep2E_0fff (@fold_rep2E_ff1f (fst (proj1_sig B))) @if_F_eq_dec_if_F_eqb compare_enc (if_map unRep) (fun T => Let_app2_In (T := T) unRep unRep) @F_pow_2_r @unfoldDiv : EdDSA_opts.
-  Hint Rewrite <- unifiedAddM1Rep_correct erep2trep_correct (fun x y z bound => iter_op_proj rep2E unifiedAddM1Rep unifiedAddM1' x y z N.testbit_nat bound unifiedAddM1Rep_correct) FRep2wire_correct: EdDSA_opts.
+  Local Existing Instance FqEncoding.
 
-  Lemma sharper_verify : forall pk l msg sig, { verify | verify = ed25519_verify pk l msg sig}.
+  Hint Rewrite @F_mul_0_l commute_negateExtended'_rep2E_rrfr fold_rep2E_0fff solve_for_R
+       (@fold_rep2E_ff1f (fst (proj1_sig B)))
+       (eqb_compare_encodings F_eqb F_eqb_iff (@weqb (b-1)) (@weqb_true_iff (b-1)))
+       (eqb_compare_encodings E.point_eqb E_eqb_iff (@weqb b) (@weqb_true_iff b))
+       (if_map unRep) unfold_E_sub E.opp_mul
+       (fun T => Let_app2_In (T := T) unRep unRep) @F_pow_2_r @unfoldDiv : EdDSA_opts.
+  Hint Rewrite <- unifiedAddM1Rep_correct erep2trep_correct
+       (fun x y z bound => iter_op_proj rep2E unifiedAddM1Rep unifiedAddM1' x y z N.testbit_nat bound unifiedAddM1Rep_correct)
+       FRep2wire_correct E.point_eqb_correct
+    : EdDSA_opts.
+
+  Lemma sharper_verify : forall pk l msg sig, { sherper_verify | sherper_verify = verify (n:=l) pk msg sig}.
   Proof.
-    eexists; intros.
-    cbv [ed25519_verify EdDSA.verify
-                        ed25519params curve25519params
-                        EdDSA.E EdDSA.B EdDSA.b EdDSA.l EdDSA.H
-                        EdDSA.PointEncoding EdDSA.FlEncoding EdDSA.FqEncoding].
+    eexists; cbv [EdDSA.verify]; intros.
 
-    etransitivity.
-    Focus 2.
-    { repeat match goal with
+    etransitivity. Focus 2. {
+      repeat match goal with 
              | [ |- ?x = ?x ] => reflexivity
              | _ => replace_option_match_with_option_rect
              | [ |- _ = option_rect _ _ _ _ ]
                => eapply option_rect_Proper_nd; [ intro | reflexivity.. ]
              end.
-      set_evars.
-      rewrite<- E.point_eqb_correct.
-      rewrite solve_for_R; unfold E.sub.
-      rewrite E.opp_mul.
-      let p1 := constr:(scalarMultM1_rep eq_refl) in
-      let p2 := constr:(unifiedAddM1_rep eq_refl) in
-      repeat match goal with
-             | |- context [(_ * E.opp ?P)%E] =>
-               rewrite <-(unExtendedPoint_mkExtendedPoint P);
-                 rewrite negateExtended_correct;
-                 rewrite <-p1
-             | |- context [(_ * ?P)%E] =>
-               rewrite <-(unExtendedPoint_mkExtendedPoint P);
-                 rewrite <-p1
-             | _ => rewrite p2
-             end;
-        rewrite ?Znat.Z_nat_N, <-?Word.wordToN_nat;
-        subst_evars;
-        reflexivity.
-    } Unfocus.
+      reflexivity. } Unfocus.
+    
+    setoid_rewrite <-E.point_eqb_correct.
+    setoid_rewrite solve_for_R.
+    setoid_rewrite (compare_without_decoding PointEncoding _ E_eqb_iff _ (@weqb_true_iff _)).
+
+    rewrite_strat bottomup hints EdDSA_opts.
+
+    setoid_rewrite <-(unExtendedPoint_mkExtendedPoint B).
+    setoid_rewrite <-(fun a => unExtendedPoint_mkExtendedPoint (E.opp a)).
+
+    setoid_rewrite <-Znat.Z_N_nat.
+    Axiom nonequivalent_optimization_Hmodl : forall n (x:word n) A, (wordToNat (H x) * A = (wordToNat (H x) mod l * A))%E.
+    setoid_rewrite nonequivalent_optimization_Hmodl.
+    setoid_rewrite <-(Nat2N.id (_ mod EdDSA.l)).
+    setoid_rewrite <-rcSOK.
+    setoid_rewrite <-(scalarMultExtendedSRep_correct _ _ _ (Fl_SRep_bound _)).
+
+    rewrite N_of_nat_modulo by (pose proof l_odd; omega).
+    
+    setoid_rewrite (unifiedAddM1_rep a_is_minus1).
 
     etransitivity.
     Focus 2.
@@ -423,12 +553,6 @@ Section Ed25519Frep.
       reflexivity.
     } Unfocus.
     rewrite <-decode_scalar_correct.
-
-    etransitivity.
-    Focus 2.
-    { do 2 (eapply option_rect_Proper_nd; [intro|reflexivity..]).
-      symmetry; apply decode_test_encode_test.
-    } Unfocus.
 
     rewrite enc'_correct.
     cbv [unExtendedPoint unifiedAddM1 negateExtended scalarMultM1].
@@ -578,4 +702,4 @@ Section Ed25519Frep.
       reflexivity. } Unfocus.
     reflexivity.
   Defined.
-End Ed25519Frep.
+End EdDSADerivation.
